add exceptions update ev ere program

src/program.v
@@ -6,12 +6,13 @@ From Coq Require Import ZArith.ZArith Strings.String.
 
 From mathcomp Require Import all_ssreflect.
 
-Require Import common_definitions bitsops bitsrep instr.
+Require Import common_definitions exceptions bitsops bitsrep instr.
 
 
 (*=Program *)
 Definition Program := seq BYTE.
 (*=End *)
+
 
 (*---------------------------------------------------------------------
  Initilize.
@@ -44,15 +45,13 @@ Definition getCodeAt (pc : EVMWORD) (pro : Program) : option BYTE :=
 Definition addBYTECode (b : BYTE) (pro : Program) : Program :=
   rcons pro b.
   
+
 (*---------------------------------------------------------------------
  Program decoder: from Hex string to Program.
  ---------------------------------------------------------------------*)
 Import Ascii.
 
-(* From BITS n to Program 
-   Return None (it is not well-formed) if the given sequence of bits 
-   is not divided into sequence of bytes
- *)
+(* From BITS n to Program, return None if the given sequence of bits is not divided into sequence of bytes *)
 Fixpoint BITStoProgram {n} :=
   match n return BITS n -> Program -> option Program with
     | 0 => fun p pro => Some pro
@@ -69,21 +68,44 @@ Fixpoint BITStoProgram {n} :=
   end.
 
 
-Definition HexToProgram s : option Program :=
-  match (BITStoProgram (fromHex s) nil) with
-    | None => None
-    | Some p => Some (rev p)
-  end.
-  
 
 (*---------------------------------------------------------------------
- Check a program is well-formed.
  A program is well-formed if
  + It is a sequence of bytes
  + For any byte that is not data of any PUSH instruction, it must be 
    valid OpCode
  + For any PUSH instruction, the number of bytes data is correct
  ---------------------------------------------------------------------*)
+Fixpoint checkwellformedProgramAux (pro : Program) (res : bool) : bool :=
+  match pro with
+    | nil => res
+    | b1::pro1 => let bopcode := BYTEToOpCode b1 in
+                  match bopcode with
+                    | BADINSTR => false
+                    | _ => let i_nat := toNat b1 in
+                           if (i_nat > 95) && (i_nat < 128) then
+                             if (size pro1) < (i_nat - 95) then
+                               false
+                             else
+                               checkwellformedProgramAux (drop (i_nat - 95) pro1) res
+                           else
+                             checkwellformedProgramAux pro1 res
+                  end
+  end.
+
+Definition checkwellformedProgram (pro : Program) :=
+  checkwellformedProgramAux pro true.
+
+
+Definition hexToProgram (s : string) : (option EVMException) * (option Program) :=
+  match (BITStoProgram (fromHex s) nil) with
+    | None => (Some BadFormProgram, None)
+    | Some p => if checkwellformedProgram (rev p) then
+                  (None, Some (rev p))
+                else
+                  (Some BadFormProgram, None)
+  end.
+  
 
 
 (*---------------------------------------------------------------------
@@ -99,217 +121,63 @@ Definition programToString (pro : Program) :=
 
 
 (*---------------------------------------------------------------------
- EVM Assembly decoder. Notice that the program should be checked 
- for well-formed one first. 
- From Bytecode to OpCode.
+ EVM Assembly decoder from binary program to opcode. 
+ Notice that the program should be well-formed.
  ---------------------------------------------------------------------*)
-
-(* The trivial implementation. However, it may helps the Proof more efficient *)
-(* Fixpoint enumProgramDecoding (pro : Program) :=
-  (if pro is b1::pro1 then
-     let i := BYTEToOpCode b1 in
-     match i with
-       | PUSH1 => match pro1 with
-                    | b2::pro2 => (instrToString i) ++ " " ++ (toHex b2) ++ " " ++ enumProgramDecoding pro2
-                    | nil => "Ill-formed program"
-                  end
-                    
-       | PUSH2 => match pro1 with
-                    | b2::b3::pro3 => (instrToString i) ++ " " ++ (toHex b2) ++ " " ++ (toHex b3) ++ " "  ++ enumProgramDecoding pro3
-                    | b2::nil => "Ill-formed program"
-                    | nil => "Ill-formed program"
-                  end
-       | PUSH3 => if (size pro1) < 3 then
-                    "Ill-formed program"
+Fixpoint assemblyDecorderAux (pro : Program) :=
+  (match pro with
+    | nil => ""
+    | b1::pro1 => let i_nat := toNat b1 in
+                  if (i_nat > 95) && (i_nat < 128) then
+                    (instrToString (BYTEToOpCode b1)) ++ " " ++ (programToString (take (i_nat - 95) pro1)) ++ assemblyDecorderAux (drop (i_nat - 95) pro1)
                   else
-                    (instrToString i) ++ " " ++ (programToString (take 3 pro1)) ++ enumProgramDecoding (drop 3 pro1)
-
-       | PUSH4 => if (size pro1) < 4 then
-                    "Ill-formed program"
-                  else
-                    (instrToString i) ++ " " ++ (programToString (take 4 pro1)) ++ enumProgramDecoding (drop 4 pro1)
-
-       | PUSH5 => if (size pro1) < 5 then
-                    "Ill-formed program"
-                  else
-                    (instrToString i) ++ " " ++ (programToString (take 5 pro1)) ++ enumProgramDecoding (drop 5 pro1)
-
-       | PUSH6 => if (size pro1) < 6 then
-                    "Ill-formed program"
-                  else
-                    (instrToString i) ++ " " ++ (programToString (take 6 pro1)) ++ enumProgramDecoding (drop 6 pro1)
-
-       | PUSH7 => if (size pro1) < 7 then
-                    "Ill-formed program"
-                  else
-                    (instrToString i) ++ " " ++ (programToString (take 7 pro1)) ++ enumProgramDecoding (drop 7 pro1)
-
-       | PUSH8 => if (size pro1) < 8 then
-                    "Ill-formed program"
-                  else
-                    (instrToString i) ++ " " ++ (programToString (take 8 pro1)) ++ enumProgramDecoding (drop 8 pro1)
-
-       | PUSH9 => if (size pro1) < 9 then
-                    "Ill-formed program"
-                  else
-                    (instrToString i) ++ " " ++ (programToString (take 9 pro1)) ++ enumProgramDecoding (drop 9 pro1)
-
-       | PUSH10 => if (size pro1) < 10 then
-                    "Ill-formed program"
-                  else
-                    (instrToString i) ++ " " ++ (programToString (take 10 pro1)) ++ enumProgramDecoding (drop 10 pro1)
-
-       | PUSH11 => if (size pro1) < 11 then
-                    "Ill-formed program"
-                  else
-                    (instrToString i) ++ " " ++ (programToString (take 11 pro1)) ++ enumProgramDecoding (drop 11 pro1)
-
-       | PUSH12 => if (size pro1) < 12 then
-                    "Ill-formed program"
-                  else
-                    (instrToString i) ++ " " ++ (programToString (take 12 pro1)) ++ enumProgramDecoding (drop 12 pro1)
-
-       | PUSH13 => if (size pro1) < 13 then
-                    "Ill-formed program"
-                  else
-                    (instrToString i) ++ " " ++ (programToString (take 13 pro1)) ++ enumProgramDecoding (drop 13 pro1)
-       | PUSH14 => if (size pro1) < 14 then
-                    "Ill-formed program"
-                  else
-                    (instrToString i) ++ " " ++ (programToString (take 14 pro1)) ++ enumProgramDecoding (drop 14 pro1)
-       | PUSH15 => if (size pro1) < 15 then
-                    "Ill-formed program"
-                  else
-                    (instrToString i) ++ " " ++ (programToString (take 15 pro1)) ++ enumProgramDecoding (drop 15 pro1)
-       | PUSH16 => if (size pro1) < 16 then
-                    "Ill-formed program"
-                  else
-                    (instrToString i) ++ " " ++ (programToString (take 16 pro1)) ++ enumProgramDecoding (drop 16 pro1)
-       | PUSH17 => if (size pro1) < 17 then
-                    "Ill-formed program"
-                  else
-                    (instrToString i) ++ " " ++ (programToString (take 17 pro1)) ++ enumProgramDecoding (drop 17 pro1)
-       | PUSH18 => if (size pro1) < 18 then
-                    "Ill-formed program"
-                  else
-                    (instrToString i) ++ " " ++ (programToString (take 18 pro1)) ++ enumProgramDecoding (drop 18 pro1)
-       | PUSH19 => if (size pro1) < 19 then
-                    "Ill-formed program"
-                  else
-                    (instrToString i) ++ " " ++ (programToString (take 19 pro1)) ++ enumProgramDecoding (drop 19 pro1)
-       | PUSH20 => if (size pro1) < 20 then
-                    "Ill-formed program"
-                  else
-                    (instrToString i) ++ " " ++ (programToString (take 20 pro1)) ++ enumProgramDecoding (drop 20 pro1)
-       | PUSH21 => if (size pro1) < 21 then
-                    "Ill-formed program"
-                  else
-                    (instrToString i) ++ " " ++ (programToString (take 21 pro1)) ++ enumProgramDecoding (drop 21 pro1)
-       | PUSH22 => if (size pro1) < 22 then
-                    "Ill-formed program"
-                  else
-                    (instrToString i) ++ " " ++ (programToString (take 22 pro1)) ++ enumProgramDecoding (drop 22 pro1)
-       | PUSH23 => if (size pro1) < 23 then
-                    "Ill-formed program"
-                  else
-                    (instrToString i) ++ " " ++ (programToString (take 23 pro1)) ++ enumProgramDecoding (drop 23 pro1)
-       | PUSH24 => if (size pro1) < 24 then
-                    "Ill-formed program"
-                  else
-                    (instrToString i) ++ " " ++ (programToString (take 24 pro1)) ++ enumProgramDecoding (drop 24 pro1)
-       | PUSH25 => if (size pro1) < 25 then
-                    "Ill-formed program"
-                  else
-                    (instrToString i) ++ " " ++ (programToString (take 25 pro1)) ++ enumProgramDecoding (drop 25 pro1)
-       | PUSH26 => if (size pro1) < 26 then
-                    "Ill-formed program"
-                  else
-                    (instrToString i) ++ " " ++ (programToString (take 26 pro1)) ++ enumProgramDecoding (drop 26 pro1)
-       | PUSH27 => if (size pro1) < 27 then
-                    "Ill-formed program"
-                  else
-                    (instrToString i) ++ " " ++ (programToString (take 27 pro1)) ++ enumProgramDecoding (drop 27 pro1)
-       | PUSH28 => if (size pro1) < 28 then
-                    "Ill-formed program"
-                  else
-                    (instrToString i) ++ " " ++ (programToString (take 28 pro1)) ++ enumProgramDecoding (drop 28 pro1)
-       | PUSH29 => if (size pro1) < 29 then
-                    "Ill-formed program"
-                  else
-                    (instrToString i) ++ " " ++ (programToString (take 29 pro1)) ++ enumProgramDecoding (drop 29 pro1)
-       | PUSH30 => if (size pro1) < 30 then
-                    "Ill-formed program"
-                  else
-                    (instrToString i) ++ " " ++ (programToString (take 30 pro1)) ++ enumProgramDecoding (drop 30 pro1)
-       | PUSH31 => if (size pro1) < 31 then
-                    "Ill-formed program"
-                  else
-                    (instrToString i) ++ " " ++ (programToString (take 31 pro1)) ++ enumProgramDecoding (drop 31 pro1)
-       | PUSH32 => if (size pro1) < 32 then
-                    "Ill-formed program"
-                  else
-                    (instrToString i) ++ " " ++ (programToString (take 32 pro1)) ++ enumProgramDecoding (drop 32 pro1)
-       
-       
-       | _ => (instrToString i) ++ " " ++ enumProgramDecoding pro1
-     end
-   else
-     "")%string.
- *)
-
-Fixpoint enumProgramDecoding (pro : Program) :=
-  (if pro is b1::pro1 then
-     let i_nat := toNat b1 in
-     (* b1 is PUSH instruction *)
-     if (i_nat > 95) && (i_nat < 128) then
-       if (size pro1) < (i_nat - 95) then
-         "Ill-formed program"
-       else
-         (instrToString (BYTEToOpCode b1)) ++ " " ++ (programToString (take (i_nat - 95) pro1)) ++ enumProgramDecoding (drop (i_nat - 95) pro1)
-     (* other instruction *)
-     else
-       (instrToString (BYTEToOpCode b1)) ++ " " ++ enumProgramDecoding pro1
-   else
-     "")%string.
+                    (instrToString (BYTEToOpCode b1)) ++ " " ++ assemblyDecorderAux pro1
+  end)%string.
 
 
-Definition AssemblyDecoder (pro : Program) :=
-  enumProgramDecoding pro.
+Definition assemblyDecoder (pro : Program) :=
+  assemblyDecorderAux pro.
 
-                                     
+
 (*---------------------------------------------------------------------
  Unit test.
  ---------------------------------------------------------------------*)
-
-
 Example hexpro1 := "6000355419600957005B72000000000000000000000000000000000000203560003555"%string.
 
-Example pro1 := HexToProgram hexpro1.
+Example pro1 := hexToProgram hexpro1.
 
 Compute (
     match pro1 with
-      | None => "Ill-formed program"%string
-      | Some p => programToString p
+      | (_, None) => "Ill-formed program"%string
+      | (_, Some p) => programToString p
     end
   ).
 
 Compute (
     match pro1 with
-      | None => "Ill-formed program"%string
-      | Some p => AssemblyDecoder p
+      | (_, None) => "Ill-formed program"%string
+      | (_, Some p) => assemblyDecoder p
     end
   ).
 
 Example hexpro2 := "6060604052609b8060106000396000f360606040526000357c0100000000000000000000000000000000000000000000000000000000900480632fbff5f3146037576035565b005b605460048080359060200190919080359060200190919050506056565b005b6000600060005060008481526020019081526020016000206000505414156096578060006000506000848152602001908152602001600020600050819055505b5b505056"%string.
 
-Example pro2 := HexToProgram hexpro2.
+Example pro2 := hexToProgram hexpro2.
 
 Compute (
     match pro2 with
-      | None => "Ill-formed program"%string
-      | Some p => AssemblyDecoder p
+      | (_, None) => "Ill-formed program"%string
+      | (_, Some p) => assemblyDecoder p
     end
   ).
 
+Example badhexpro := hexToProgram "6060604052609b8060106000396000f360606040526000357c010000000000000000"%string.
+
+Compute (
+    match badhexpro with
+      | (_, None) => "Ill-formed program"%string
+      | (_, Some p) => assemblyDecoder p
+    end
+  ).
 
 	
