src/exceptions.v
@@ -1,0 +1,27 @@
+(*===================================================================================================================================================================================
+ All EVM exceptions.
+ ===================================================================================================================================================================================*)
+
+Require Import mathcomp.ssreflect.ssreflect.
+From mathcomp Require Import ssrfun ssrbool eqtype ssrnat seq fintype finfun tuple zmodp.
+
+Require Import common_definitions.
+
+Set Implicit Arguments.
+Unset Strict Implicit.
+Import Prenex Implicits.
+
+
+
+(*=EVM Exception *)
+Inductive EVMException :=
+| BreakPointHit
+| BadInstruction
+| BadJumpDestination
+| OutOfGas
+| OutOfStack              (* e.g. peek an item when the stack is empty *)
+| StackUnderflow
+| StackOverflow
+| BadFormProgram
+| OutOfRange.             (* e.g. get a byte code at a position beyon the program bytecode *)
+(*=End *)
